GenInd.v
@@ -1,6 +1,7 @@
 From Ltac2 Require Import Ltac2.
 
 Require Import List.
+Require Import Rewrite.
 Require Import Misc.
 
 Ltac2 eassumption_tac () := ltac1:(eassumption).
@@ -24,6 +25,132 @@ Proof.
   intros x Hx; split > [apply Hx|apply H1, Hx].
 Defined.
 
+Lemma Forall3_impl_transparent :
+  forall (A B C : Type) (P Q : A -> B -> C -> Prop) (l1 : list A) (l2 : list B) (l3 : list C), (forall x y z, P x y z -> Q x y z) -> Forall3 P l1 l2 l3 -> Forall3 Q l1 l2 l3.
+Proof.
+  intros A B C P Q l1 l2 l3 H1 H2; induction H2; constructor.
+  - apply H1. assumption.
+  - assumption.
+Defined.
+
+Inductive if_Some {A : Type} (P : A -> Prop) : option A -> Prop :=
+| if_Some_None : if_Some P None
+| if_Some_Some : forall x, P x -> if_Some P (Some x).
+
+Lemma if_Some_impl_transparent :
+  forall (A : Type) (P Q : A -> Prop) (x : option A), (forall x, P x -> Q x) -> if_Some P x -> if_Some Q x.
+Proof.
+  intros A P Q x H1 H2. inversion H2; subst.
+  - constructor.
+  - constructor; apply H1. assumption.
+Defined.
+
+Inductive if_Some2 {A B : Type} (P : A -> B -> Prop) : option A -> option B -> Prop :=
+| if_Some2_None : if_Some2 P None None
+| if_Some2_Some : forall x y, P x y -> if_Some2 P (Some x) (Some y).
+
+Lemma if_Some2_impl_transparent :
+  forall (A B : Type) (P Q : A -> B -> Prop) (x : option A) (y : option B), (forall x y, P x y -> Q x y) -> if_Some2 P x y -> if_Some2 Q x y.
+Proof.
+  intros A B P Q x y H1 H2. inversion H2; subst.
+  - constructor.
+  - constructor; apply H1. assumption.
+Defined.
+
+Inductive if_Some3 {A B C : Type} (P : A -> B -> C -> Prop) : option A -> option B -> option C -> Prop :=
+| if_Some3_None : if_Some3 P None None None
+| if_Some3_Some : forall x y z, P x y z -> if_Some3 P (Some x) (Some y) (Some z).
+
+Lemma if_Some3_impl_transparent :
+  forall (A B C : Type) (P Q : A -> B -> C -> Prop) (x : option A) (y : option B) (z : option C), (forall x y z, P x y z -> Q x y z) -> if_Some3 P x y z -> if_Some3 Q x y z.
+Proof.
+  intros A B C P Q x y z H1 H2. inversion H2; subst.
+  - constructor.
+  - constructor; apply H1. assumption.
+Defined.
+
+
+(*
+Lemma exists_impl_transparent :
+  forall (A : Type) (P Q : A -> Prop), (exists x, P x) -> (forall x, P x -> Q x) -> (exists x, Q x).
+Proof.
+  intros A P Q [x H1] H2. exists x. apply H2, H1.
+Defined.
+
+Lemma exists_impl_strong_transparent :
+  forall (A : Type) (P Q : A -> Prop), (exists x, P x) -> (forall x, P x -> Q x) -> (exists x, P x /\ Q x).
+Proof.
+  intros A P Q H1 H2. eapply exists_impl_transparent > [eassumption|].
+  intros x Hx; split > [apply Hx|apply H2, Hx].
+Defined.
+*)
+
+Ltac2 msg_list_concat (l : message list) (sep : message) :=
+  match l with
+  | [] => Message.of_string ""
+  | x :: l => List.fold_left (fun m x => Message.concat m (Message.concat sep x)) l x
+  end.
+
+Ltac2 message_concat_list (l : message list) :=
+  List.fold_left (fun m1 m2 => Message.concat m1 m2) l (Message.of_string "").
+
+Ltac2 message_of_hyps () :=
+  message_concat_list (List.map (fun (id, _, c) => message_concat_list [Message.of_ident id; Message.of_string " : "; Message.of_constr c; Message.of_string "
+"]) (Control.hyps ())).
+
+Ltac2 typed_constr_message (c : constr) :=
+  Message.concat (Message.concat (Message.of_constr c) (Message.of_string " : ")) (Message.of_constr (Constr.type c)).
+
+Ltac2 msg_of_binder (b : binder) :=
+  Message.concat
+    (match Constr.Binder.name b with None => Message.of_string "_" | Some x => Message.of_ident x end)
+    (Message.concat (Message.of_string " : ")
+                    (typed_constr_message (Constr.Binder.type b))).
+
+Ltac2 msg_of_list (l : message list) :=
+  message_concat_list [Message.of_string "[" ; msg_list_concat l (Message.of_string "; "); Message.of_string "]"].
+
+Ltac2 msg_of_array (a : message array) :=
+  message_concat_list [Message.of_string "[|" ; msg_list_concat (Array.to_list a) (Message.of_string "; "); Message.of_string "|]"].
+
+Ltac2 show_constr_kind (c : constr) :=
+  let sp := Message.of_string " " in
+  match Constr.Unsafe.kind c with
+  | Constr.Unsafe.Rel n => Message.concat (Message.of_string "Rel ") (Message.of_int n)
+  | Constr.Unsafe.Var x => Message.concat (Message.of_string "Var ") (Message.of_ident x)
+  | Constr.Unsafe.Meta _ => Message.of_string "Meta _"
+  | Constr.Unsafe.Evar e ca => Message.concat (Message.of_string "Evar _ ") (msg_of_array (Array.map Message.of_constr ca))
+  | Constr.Unsafe.Sort _ => Message.of_string "Sort _"
+  | Constr.Unsafe.Cast c1 _ c2 => message_concat_list [Message.of_string "Cast " ; Message.of_constr c1 ; Message.of_string " _ " ; Message.of_constr c2]
+  | Constr.Unsafe.Prod b c => message_concat_list [Message.of_string "Prod " ; msg_of_binder b ; sp ; Message.of_constr c]
+  | Constr.Unsafe.Lambda  b c => message_concat_list [Message.of_string "Lambda " ; msg_of_binder b ; sp ; Message.of_constr c]
+  | Constr.Unsafe.LetIn b c1 c2 => message_concat_list [Message.of_string "LetIn " ; msg_of_binder b ; sp ; Message.of_constr c1 ; sp ; Message.of_constr c2]
+  | Constr.Unsafe.App c ca => message_concat_list [Message.of_string "App " ; Message.of_constr c ; sp; msg_of_array (Array.map Message.of_constr ca)]
+  | Constr.Unsafe.Constant _ _ => Message.of_string "Constant _ _"
+  | Constr.Unsafe.Ind _ _ => Message.of_string "Ind _ _"
+  | Constr.Unsafe.Constructor _ _ => Message.of_string "Constructor _ _"
+  | Constr.Unsafe.Case _ c1 ci c2 ca => message_concat_list [Message.of_string "Case _ " ; Message.of_constr c1 ; sp ; match ci with Constr.Unsafe.NoInvert => Message.of_string "NoInvert" | Constr.Unsafe.CaseInvert ca => message_concat_list [Message.of_string "(CaseInvert "; msg_of_array (Array.map Message.of_constr ca); Message.of_string ")"] end ; sp ; Message.of_constr c2 ; sp ; msg_of_array (Array.map Message.of_constr ca) ]
+  | Constr.Unsafe.Fix ia i ba ca => message_concat_list [Message.of_string "Fix "; msg_of_array (Array.map Message.of_int ia); sp ; Message.of_int i ; sp ; msg_of_array (Array.map msg_of_binder ba) ; sp ; msg_of_array (Array.map Message.of_constr ca)]
+  | Constr.Unsafe.CoFix i ba ca => message_concat_list [Message.of_string "CoFix "; Message.of_int i ; sp ; msg_of_array (Array.map msg_of_binder ba) ; sp ; msg_of_array (Array.map Message.of_constr ca)]
+  | Constr.Unsafe.Proj _ c => message_concat_list [Message.of_string "Proj _ "; Message.of_constr c]
+  | Constr.Unsafe.Uint63 _ => Message.of_string "Uint63 _"
+  | Constr.Unsafe.Float _ => Message.of_string "Float _"
+  | Constr.Unsafe.Array _ ca c1 c2 => message_concat_list [Message.of_string "Array _ "; msg_of_array (Array.map Message.of_constr ca) ; sp ; Message.of_constr c1 ; sp ; Message.of_constr c2]
+  end.
+(*
+Inductive even : nat -> Prop :=
+| even_O : even O
+| even_SS : forall n, even n -> even (S (S n)).
+Print even_ind.
+(*Fixpoint t (n : nat) (H : even n) : Prop :=
+  match H return Prop with
+  | even_O => n = n
+  | even_SS n H1 => t n H1
+  end.*)
+Goal True.
+  let tdef := Std.eval_cbv {Std.rBeta := true ; Std.rMatch := false ; Std.rFix := false ; Std.rCofix := false ; Std.rZeta := false ; Std.rDelta := true ; Std.rConst := []} '(even_ind (fun n => even n) even_O (fun n _ Hrec => even_SS n Hrec)) in
+  Message.print (show_constr_kind tdef).
+*)
 Ltac2 get_binder_maybe (c : constr) :=
   match Constr.Unsafe.kind c with
   | Constr.Unsafe.Prod b _ => Some b
@@ -55,8 +182,23 @@ Ltac2 rec rebuild_lam (t : constr) :=
   | _ => t
   end.
 
+Ltac2 rec rebuild_prod_cast (t : constr) :=
+  match Constr.Unsafe.kind t with
+  | Constr.Unsafe.Prod b t1 => Constr.Unsafe.make (Constr.Unsafe.Prod b (rebuild_prod_cast t1))
+  | Constr.Unsafe.Lambda b t1 => Constr.Unsafe.make (Constr.Unsafe.Lambda b (rebuild_prod_cast t1))
+  | Constr.Unsafe.Cast t1 _ _ => rebuild_prod_cast t1
+  | _ => t
+  end.
+
+Ltac2 force_prop (tac : unit -> constr) :=
+  '(ltac2:(Control.refine tac) : Prop).
+Ltac2 force_prop_t (tac : unit -> constr) :=
+  '(ltac2:(Control.refine tac) : _ : Prop).
+
 Ltac2 inctx (name : ident) (t : constr) (body : constr -> constr) :=
-  Constr.in_context name t (fun () => Control.refine (fun () => body (Control.hyp name))).
+  rebuild_lam (Constr.in_context name t (fun () => Control.refine (fun () => body (Control.hyp name)))).
+Ltac2 inctx_p (name : ident) (t : constr) (body : constr -> constr) :=
+  force_prop_t (fun () => inctx name t body).
 
 Ltac2 make_forall (c : constr) :=
   match Constr.Unsafe.kind c with
@@ -72,7 +214,7 @@ Ltac2 mk_forall_proof_smart (x : ident) (u : constr) (v : constr -> constr) :=
   lazy_match! (Std.eval_hnf u) with
   | True => v 'I
   | ?u =>
-    let vx := inctx x u v in
+    let vx := inctx_p x u v in
     lazy_match! (Std.eval_hnf (Constr.type vx)) with
     | (_ -> True) => 'I
     | _ => vx
@@ -80,7 +222,7 @@ Ltac2 mk_forall_proof_smart (x : ident) (u : constr) (v : constr -> constr) :=
   end.
 
 Ltac2 mk_Forall_proof_smart (x : ident) (t : constr) (u : constr -> constr) (v : constr) :=
-  let ux := inctx x t u in
+  let ux := inctx_p x t u in
   lazy_match! (Std.eval_hnf (Constr.type ux)) with
   | (_ -> True) => 'I
   | _ => '(Forall_True_transparent $t _ $v $ux)
@@ -92,44 +234,96 @@ Ltac2 mk_and_proof_smart (u : constr) (v : constr) :=
   lazy_match! '($ut /\ $vt) with
   | True /\ _ => v
   | _ /\ True => u
-  | _ => '(conj _ _ $u $v)
+  | _ => '(conj $u $v)
   end.
 
 
 Ltac2 mk_Forall_impl_smart (t : constr) (p : constr) (l : constr) (u : constr -> constr) (v : constr) :=
-  let ux := inctx (head_binder_ident p) t (fun xx => inctx (Fresh.in_goal @H) (mk_app p xx) u) in
+  let ux := inctx_p (head_binder_ident p) t (fun xx => inctx (Fresh.in_goal @H) (mk_app p xx) u) in
   lazy_match! (Std.eval_hnf (Constr.type ux)) with
   | (forall x H, True) => 'I
   | _ => '(Forall_impl_transparent $t _ _ $l $ux $v)
   end.
 
 Ltac2 mk_Forall2_impl_smart (t1 : constr) (t2 : constr) (p : constr) (l1 : constr) (l2 : constr) (u : constr -> constr) (v : constr) :=
-  let ux := inctx (head_binder_ident p) t1 (fun xx =>
+  let ux := inctx_p (head_binder_ident p) t1 (fun xx =>
     let y := head_binder_ident (Std.eval_hnf (mk_app p xx)) in
-    inctx y t2 (fun yy =>
-      inctx (Fresh.in_goal @H) (mk_app (mk_app p xx) yy) u)) in
+    inctx_p y t2 (fun yy =>
+      inctx_p (Fresh.in_goal @H) (mk_app (mk_app p xx) yy) u)) in
   lazy_match! (Std.eval_hnf (Constr.type ux)) with
   | (forall x y H, True) => 'I
   | _ => '(Forall2_impl_transparent $t1 $t2 _ _ $l1 $l2 $ux $v)
   end.
 
+Ltac2 mk_Forall3_impl_smart (t1 : constr) (t2 : constr) (t3 : constr) (p : constr) (l1 : constr) (l2 : constr) (l3 : constr) (u : constr -> constr) (v : constr) :=
+  let ux := inctx_p (head_binder_ident p) t1 (fun xx =>
+    let y := head_binder_ident (Std.eval_hnf (mk_app p xx)) in
+    inctx_p y t2 (fun yy =>
+      let z := head_binder_ident (Std.eval_hnf (mk_app (mk_app p xx) yy)) in
+      inctx_p z t3 (fun zz =>
+        inctx_p (Fresh.in_goal @H) (mk_app (mk_app (mk_app p xx) yy) zz) u))) in
+  lazy_match! (Std.eval_hnf (Constr.type ux)) with
+  | (forall x y z H, True) => 'I
+  | _ => '(Forall3_impl_transparent $t1 $t2 $t3 _ _ $l1 $l2 $l3 $ux $v)
+  end.
+
+Ltac2 mk_if_Some_impl_smart (t : constr) (p : constr) (o : constr) (u : constr -> constr) (v : constr) :=
+  let ux := inctx_p (head_binder_ident p) t (fun xx => inctx (Fresh.in_goal @H) (mk_app p xx) u) in
+  lazy_match! (Std.eval_hnf (Constr.type ux)) with
+  | (forall x H, True) => 'I
+  | _ => '(if_Some_impl_transparent $t _ _ $o $ux $v)
+  end.
+
+Ltac2 mk_if_Some2_impl_smart (t1 : constr) (t2 : constr) (p : constr) (o1 : constr) (o2 : constr) (u : constr -> constr) (v : constr) :=
+  let ux := inctx_p (head_binder_ident p) t1 (fun xx =>
+    let y := head_binder_ident (Std.eval_hnf (mk_app p xx)) in
+    inctx_p y t2 (fun yy =>
+      inctx_p (Fresh.in_goal @H) (mk_app (mk_app p xx) yy) u)) in
+  lazy_match! (Std.eval_hnf (Constr.type ux)) with
+  | (forall x y H, True) => 'I
+  | _ => '(if_Some2_impl_transparent $t1 $t2 _ _ $o1 $o2 $ux $v)
+  end.
+
+Ltac2 mk_if_Some3_impl_smart (t1 : constr) (t2 : constr) (t3 : constr) (p : constr) (o1 : constr) (o2 : constr) (o3 : constr) (u : constr -> constr) (v : constr) :=
+  let ux := inctx_p (head_binder_ident p) t1 (fun xx =>
+    let y := head_binder_ident (Std.eval_hnf (mk_app p xx)) in
+    inctx_p y t2 (fun yy =>
+      let z := head_binder_ident (Std.eval_hnf (mk_app (mk_app p xx) yy)) in
+      inctx_p z t3 (fun zz =>
+        inctx_p (Fresh.in_goal @H) (mk_app (mk_app (mk_app p xx) yy) zz) u))) in
+  lazy_match! (Std.eval_hnf (Constr.type ux)) with
+  | (forall x y z H, True) => 'I
+  | _ => '(if_Some3_impl_transparent $t1 $t2 $t3 _ _ $o1 $o2 $o3 $ux $v)
+  end.
+
+
+Ltac2 mk_step_one_impl_smart (t : constr) (r : constr) (l1 : constr) (l2 : constr) (u : constr -> constr) (v : constr) :=
+  let ux := inctx_p (head_binder_ident r) t (fun xx =>
+    let y := head_binder_ident (Std.eval_hnf (mk_app r xx)) in
+    inctx_p y t (fun yy =>
+      inctx_p (Fresh.in_goal @H) (mk_app (mk_app r xx) yy) u)) in
+  lazy_match! (Std.eval_hnf (Constr.type ux)) with
+  | (forall x y H, True) => 'I
+  | _ => '(step_one_impl_strong_transparent $t _ _ $l1 $l2 $ux $v)
+  end.
+
 Ltac2 mk_Exists_impl_smart (t : constr) (p : constr) (l : constr) (u : constr -> constr) (v : constr) :=
-  let ux := inctx (head_binder_ident p) t (fun xx => inctx (Fresh.in_goal @H) (mk_app p xx) u) in
+  let ux := inctx_p (head_binder_ident p) t (fun xx => inctx (Fresh.in_goal @H) (mk_app p xx) u) in
   lazy_match! (Std.eval_hnf (Constr.type ux)) with
   | (forall x H, True) => 'I
   | _ => '(Exists_impl_strong_transparent $t _ _ $l $ux $v)
   end.
 
+(*
+Ltac2 mk_exists_impl_smart (t : constr) (p : constr) (u : constr -> constr) (v : constr) :=
+  let ux := inctx_p (head_binder_ident p) t (fun xx => inctx (Fresh.in_goal @H) (mk_app p xx) u) in
+  lazy_match! (Std.eval_hnf (Constr.type ux)) with
+  | (forall x H, True) => 'I
+  | _ => '(exists_impl_strong_transparent $t _ _ $ux $v)
+  end.
+ *)
 
-Ltac2 message_concat_list (l : message list) :=
-  List.fold_left (fun m1 m2 => Message.concat m1 m2) l (Message.of_string "").
 
-Ltac2 message_of_hyps () :=
-  message_concat_list (List.map (fun (id, _, c) => message_concat_list [Message.of_ident id; Message.of_string " : "; Message.of_constr c; Message.of_string "
-"]) (Control.hyps ())).
-
-Ltac2 typed_constr_message (c : constr) :=
-  Message.concat (Message.concat (Message.of_constr c) (Message.of_string " : ")) (Message.of_constr (Constr.type c)).
 Ltac2 log (c : constr) := Message.print (typed_constr_message c).
 Ltac2 logged (r : constr) := log r; r.
 Ltac2 log_context () := Message.print (Message.of_string "Context:"); Message.print (message_of_hyps ()).
@@ -171,8 +365,20 @@ Ltac2 rec constrind_hyp (v : constr) (inds : constr list) (hrecs : constr list) 
       mk_Forall_impl_smart t p l (fun h => constrind_hyp h inds hrecs) v
     | @Forall2 ?t1 ?t2 ?p ?l1 ?l2 =>
       mk_Forall2_impl_smart t1 t2 p l1 l2 (fun h => constrind_hyp h inds hrecs) v
+    | @Forall3 ?t1 ?t2 ?t3 ?p ?l1 ?l2 ?l3 =>
+      mk_Forall3_impl_smart t1 t2 t3 p l1 l2 l3 (fun h => constrind_hyp h inds hrecs) v
+    | @if_Some ?t ?p ?x =>
+      mk_if_Some_impl_smart t p x (fun h => constrind_hyp h inds hrecs) v
+    | @if_Some2 ?t1 ?t2 ?p ?x ?y =>
+      mk_if_Some2_impl_smart t1 t2 p x y (fun h => constrind_hyp h inds hrecs) v
+    | @if_Some3 ?t1 ?t2 ?t3 ?p ?x ?y ?z =>
+      mk_if_Some3_impl_smart t1 t2 t3 p x y z (fun h => constrind_hyp h inds hrecs) v
+    | @step_one ?t ?r ?l1 ?l2 =>
+      mk_step_one_impl_smart t r l1 l2 (fun h => constrind_hyp h inds hrecs) v
     | @Exists ?t ?p ?l =>
       mk_Exists_impl_smart t p l (fun h => constrind_hyp h inds hrecs) v
+(*    | @ex ?t ?p =>
+      mk_exists_impl_smart t p (fun h => constrind_hyp h inds hrecs) v *)
     | (?a * ?b)%type =>
       mk_and_proof_smart
         (constrind_hyp (mk_app 'fst v) inds hrecs)
@@ -204,7 +410,7 @@ Ltac2 rec constrind1 (c : constr) (cstr : constr) (cstrhyp : constr) (inds : con
   lazy_match! c with
   | forall (x : ?t1), @?t2 x =>
     let x := head_binder_ident c in
-    inctx x t1 (fun xx =>
+    inctx_p x t1 (fun xx =>
       constrind1 (mk_app t2 xx) cstr cstrhyp inds ps hrecs (xx :: args) (add1 (constrind_hyp xx inds hrecs) args_recs)
     )
   | ?c =>
@@ -221,7 +427,7 @@ Ltac2 rec constrind1 (c : constr) (cstr : constr) (cstrhyp : constr) (inds : con
 Ltac2 get_constructors_base (ind : inductive) (inst : instance) (args : constr list) :=
   List.init (Ind.nconstructors (Ind.data ind))
             (fun i => let c := Ind.get_constructor (Ind.data ind) i in
-                   applist (Constr.Unsafe.make (Constr.Unsafe.Constructor c inst)) args
+                   applist (Constr.Unsafe.make (Constr.Unsafe.Constructor c inst)) (List.rev args)
             ).
 
 Ltac2 rec split_ind (c : constr) (args : constr list) :=
@@ -256,7 +462,7 @@ Ltac2 named_ident (s : string) := match Ident.of_string s with Some i => i | Non
 Ltac2 rec ncontext (l : constr list) (l2 : constr list) (tac : constr list -> constr) :=
   match l with
   | [] => tac (List.rev l2)
-  | _ :: l => inctx (Fresh.in_goal @H) '(_ : Prop) (fun h => ncontext l (h :: l2) tac)
+  | _ :: l => inctx_p (Fresh.in_goal @H) '(_ : Prop) (fun h => ncontext l (h :: l2) tac)
   end.
 
 Ltac2 rec nabs (n : int) (c : constr) :=
@@ -267,27 +473,29 @@ Ltac2 rec ind_principle_p (t : constr) :=
   | forall (x : ?t1), _ =>
     let x := head_binder_ident (Constr.type t) in
     make_forall (inctx x t1 (fun xx => ind_principle_p (mk_app t xx)))
-  | Set => '($t -> Prop)
-  | Type => '($t -> Prop)
+  | Set => '(($t -> Prop) : Prop)
+  | Type => '(($t -> Prop) : Prop)
   | Prop => 'Prop
   end.
 
 Ltac2 rec forall_principle (t : constr) (p : constr) :=
+  force_prop (fun () =>
   lazy_match! (Constr.type t) with
   | forall (x : ?t1), _ =>
     let x := head_binder_ident (Constr.type t) in
     make_forall (inctx x t1 (fun xx => forall_principle (mk_app t xx) (mk_app p xx)))
   | Set => '(forall (t : $t), $p t)
   | Type => '(forall (t : $t), $p t)
-  | Prop => '($t -> $p)
-end.
+  | Prop => '(($t -> $p) : Prop)
+  end).
 
 Ltac2 rec intro_hyp (name : ident) (c : constr) (tac : constr -> constr) :=
+  force_prop_t (fun () =>
   lazy_match! (Constr.type c) with
   | forall (x : ?t1), _ =>
     inctx (head_binder_ident (Constr.type c)) t1 (fun xx => intro_hyp name (mk_app c xx) tac)
   | _ => inctx name c tac
-  end.
+  end).
 
 Ltac2 rec rec_pos (t : constr) :=
   match Constr.Unsafe.kind t with
@@ -337,7 +545,9 @@ Ltac2 rec get_body (names : ident list) (bds : binder list) (t : constr) :=
     end
   end.
 
-Ltac2 mkprod u v := '($u, $v).
+(* Ltac2 mkprod u v := '(conj _ _ $u $v). *)
+Ltac2 mkprod u v :=
+  '(conj $u $v).
 
 Ltac2 rec mkprodn (l : constr list) :=
   match List.tl l with
@@ -345,13 +555,27 @@ Ltac2 rec mkprodn (l : constr list) :=
   | _ => mkprod (List.hd l) (mkprodn (List.tl l))
   end.
 
-Ltac2 mkfix (guarded_arg : int list) (names : ident list) (ts : constr list) (body : (constr list -> constr) list) :=
-  let bodies := List.map (inctxn names ts) body in
+Ltac2 rotate_left (l : 'a list) (n : int) :=
+  List.append (List.skipn n l) (List.firstn n l).
+Ltac2 rotate_right (l : 'a list) (n : int) :=
+  rotate_left l (Int.sub (List.length l) n).
+
+Ltac2 mkfix_one (guarded_arg : int list) (names : ident list) (ts : constr list) (body : (constr list -> constr) list) (n : int) :=
+  let ts := List.map rebuild_prod_cast ts in
+  let bodies := List.map rebuild_prod_cast (List.map (inctxn names ts) body) in
+  (* List.iter Message.print (List.map show_constr_kind ts);
+  List.iter log ts; List.iter log (List.map Constr.type bodies); *)
   let (binders, _) := get_body names [] (List.hd bodies) in
   let binders := Array.of_list binders in
   let guarded_arg := Array.of_list guarded_arg in
   let bodies := Array.of_list (List.map (fun body => let (_, body) := (get_body names [] body) in body) bodies) in
-  mkprodn (List.init (List.length names) (fun n => Constr.Unsafe.make (Constr.Unsafe.Fix guarded_arg n binders bodies))).
+  Constr.Unsafe.make (Constr.Unsafe.Fix guarded_arg n binders bodies).
+
+Ltac2 mkfix_one' (guarded_arg : int list) (names : ident list) (ts : constr list) (body : (constr list -> constr) list) (n : int) :=
+  mkfix_one (rotate_left guarded_arg n) (rotate_left names n) (rotate_left ts n) (rotate_left (List.map (fun f l => f (rotate_right l n)) body) n) 0.
+
+Ltac2 mkfix (guarded_arg : int list) (names : ident list) (ts : constr list) (body : (constr list -> constr) list) :=
+  mkprodn (List.init (List.length names) (fun n => mkfix_one guarded_arg names ts body n)).
 
 Ltac2 map3 f l1 l2 l3 := List.map2 (fun a (b, c) => f a b c) l1 (List.combine l2 l3).
 Ltac2 map4 f l1 l2 l3 l4 := map3 (fun a b (c, d) => f a b c d) l1 l2 (List.combine l3 l4).
@@ -366,14 +590,14 @@ Ltac2 gen_ind_principle (cl : constr list) :=
       mkfix (List.map (fun c => rec_pos (Constr.type c)) cl) (fresh_n_goal n @Hrec) (List.map2 forall_principle cl pl)
             (map5 (fun c (ind, _, _) => fun p cstrs lhyps hrecs =>
         intro_hyp (Fresh.in_goal @x) c (fun xx =>
-          let branches := List.map2 (fun cstr hcstr => rebuild_lam (constrind1 (Constr.type cstr) cstr hcstr cl pl hrecs [] [])) cstrs lhyps in
-          Constr.Unsafe.make
+          let branches := List.map2 (fun cstr hcstr => force_prop_t (fun () => rebuild_lam (constrind1 (Constr.type cstr) cstr hcstr cl pl hrecs [] []))) cstrs lhyps in log (rebuild_lam (eta_expand c p));
+          force_prop_t (fun () => Constr.Unsafe.make
             (Constr.Unsafe.Case
                (Constr.Unsafe.case ind)
                (rebuild_lam (eta_expand c p))
                Constr.Unsafe.NoInvert
                xx
-               (Array.of_list branches))
+               (Array.of_list branches)))
          )) cl indstl pl cstrsl lhypsl)
     )
   ).
@@ -387,3 +611,17 @@ Notation "'Induction' 'For' [ x ; y ; z ; w ]" :=
   ltac2:(let l := [x; y; z; w] in Control.refine (fun () => gen_ind_principle (List.map Constr.pretype l))) (at level 0, only parsing).
 Notation "'Induction' 'For' [ x ; y ; z ; w ; t ]" :=
   ltac2:(let l := [x; y; z; w; t] in Control.refine (fun () => gen_ind_principle (List.map Constr.pretype l))) (at level 0, only parsing).
+
+(*
+Inductive even : nat -> Prop :=
+| even_O : even O
+| even_SS : forall n, even n -> even (S (S n)).
+Definition a := Induction For [ even ].
+Definition b := a even even_O (fun n _ Hrec => even_SS n Hrec).
+Check b.
+Goal True.
+
+  log (Constr.type 'b).
+
+Check (forall (x : nat), Prop).
+*)
